Change compilation of top_addr in loop_to_word
TopAddr shouldn't be EndOfHeap, because EndOfHeap is the end of the
CakeML heap, which is only half of the Pancake memory.

pancake/proofs/loop_to_wordProofScript.sml
@@ -41,6 +41,7 @@ End
 
 Definition state_rel_def:
   state_rel s t <=>
+  ∃len.
     t.memory = s.memory ∧
     t.mdomain = s.mdomain ∧
     t.sh_mdomain = s.sh_mdomain ∧
@@ -48,7 +49,8 @@ Definition state_rel_def:
     t.be = s.be ∧
     t.ffi = s.ffi ∧
     ALOOKUP (fmap_to_alist t.store) CurrHeap = SOME (Word s.base_addr) ∧
-    ALOOKUP (fmap_to_alist t.store) EndOfHeap = SOME (Word s.top_addr) ∧
+    ALOOKUP (fmap_to_alist t.store) HeapLength = SOME (Word len) ∧
+    s.top_addr = s.base_addr + 2w*len ∧
     globals_rel s.globals t.store ∧
     code_rel s.code t.code
 End
@@ -57,8 +59,8 @@ val goal =
   ``λ(prog:α loopLang$prog, s). ∀res s1 t ctxt retv l.
       evaluate (prog,s) = (res,s1) ∧ res ≠ SOME Error ∧
       state_rel s t ∧ locals_rel ctxt s.locals t.locals ∧
-      ALOOKUP (fmap_to_alist t.store) CurrHeap = SOME (Word s.base_addr) ∧
-      ALOOKUP (fmap_to_alist t.store) EndOfHeap = SOME (Word s.top_addr) ∧
+(*      ALOOKUP (fmap_to_alist t.store) CurrHeap = SOME (Word s.base_addr) ∧
+      ALOOKUP (fmap_to_alist t.store) EndOfHeap = SOME (Word s.top_addr) ∧*)
       lookup 0 t.locals = SOME retv ∧ no_Loops prog ∧
       good_dimindex(:'a) ∧
       ~(isWord retv) ∧
@@ -133,7 +135,7 @@ Theorem state_rel_intro:
     globals_rel s.globals t.store ∧
     code_rel s.code t.code
 Proof
-  rw [state_rel_def]
+  rw [state_rel_def] >> simp[]
 QED
 
 Theorem find_var_neq_0:
@@ -183,7 +185,7 @@ QED
 Triviality state_rel_IMP:
   state_rel s t ⇒ t.clock = s.clock
 Proof
-  fs [state_rel_def]
+  fs [state_rel_def] >> metis_tac[]
 QED
 
 Theorem set_fromNumSet:
@@ -326,47 +328,46 @@ QED
 
 Theorem comp_exp_preserves_eval:
   !s e v t ctxt.
-   eval s e = SOME v ∧
+   eval s (e:α loopLang$exp) = SOME v ∧ good_dimindex(:'a) ∧
    state_rel s t /\ locals_rel ctxt s.locals t.locals ==>
    word_exp t (comp_exp ctxt e) = SOME v
 Proof
   ho_match_mp_tac eval_ind >>
   rw [] >>
   fs [eval_def, comp_exp_def, word_exp_def]
-  >- (
-   fs [find_var_def, locals_rel_def] >>
-   TOP_CASE_TAC >> fs [] >>
-   first_x_assum drule >>
-   strip_tac >> fs [] >> rveq >> fs [])
+  >- (fs [find_var_def, locals_rel_def] >>
+      TOP_CASE_TAC >> fs [] >>
+      first_x_assum drule >>
+      strip_tac >> fs [] >> rveq >> fs [])
   >- fs [state_rel_def, globals_rel_def]
-  >- (
-   cases_on ‘eval s e’ >> fs [] >>
-   cases_on ‘x’ >> fs [] >>
-   first_x_assum drule_all >> fs [] >>
-   strip_tac >>
-   fs [state_rel_def, mem_load_def,
-       loopSemTheory.mem_load_def])
-  >- (
-  fs [CaseEq "option"] >>
-  qsuff_tac
-  ‘the_words (MAP (λa. word_exp t a)
-              (MAP (λa. comp_exp ctxt a) wexps)) = SOME ws’
-  >- fs [] >>
-  ntac 2 (pop_assum mp_tac) >>
-  ntac 2 (pop_assum kall_tac) >>
-  rpt (pop_assum mp_tac) >>
-  qid_spec_tac ‘ws’ >>
-  qid_spec_tac ‘wexps’ >>
-  Induct >> rw [] >>
-  last_assum mp_tac >>
-  impl_tac >- metis_tac [] >>
-  fs [the_words_def, CaseEq"option", CaseEq"word_loc"] >>
-  rveq >> fs [])
+  >- (cases_on ‘eval s e’ >> fs [] >>
+      cases_on ‘x’ >> fs [] >>
+      first_x_assum drule_all >> fs [] >>
+      strip_tac >>
+      fs [state_rel_def, mem_load_def,
+      loopSemTheory.mem_load_def])
+  >- (fs [CaseEq "option"] >>
+      qsuff_tac
+      ‘the_words (MAP (λa. word_exp t a)
+                      (MAP (λa. comp_exp ctxt a) wexps)) = SOME ws’
+      >- fs [] >>
+      ntac 2 (pop_assum mp_tac) >>
+      ntac 3 (pop_assum kall_tac) >>
+      rpt (pop_assum mp_tac) >>
+      qid_spec_tac ‘ws’ >>
+      qid_spec_tac ‘wexps’ >>
+      Induct >> rw [] >>
+      last_assum mp_tac >>
+      impl_tac >- metis_tac [] >>
+      fs [the_words_def, CaseEq"option", CaseEq"word_loc"] >>
+      rveq >> fs [])
   >- (fs [CaseEq"option", CaseEq"word_loc"] >> rveq >> fs []) >>
   fs[state_rel_def] >>
   Cases_on ‘FLOOKUP t.store CurrHeap’ >> fs[] >>
   rename1 ‘x’ >>
-  Cases_on ‘x’ >> fs[theWord_def, isWord_def]
+  Cases_on ‘x’ >> fs[theWord_def, isWord_def,word_sh_def, the_words_def, good_dimindex_def,word_op_def] >>
+  gvs[] >>
+  simp[WORD_MUL_LSL]
 QED
 
 
@@ -382,7 +383,8 @@ Proof
   TOP_CASE_TAC >>
   fs [flush_state_def, state_rel_def,
       loopSemTheory.dec_clock_def, dec_clock_def] >> rveq >>
-  fs []
+  fs [] >>
+  rw[]
 QED
 
 Theorem compile_Loop:
@@ -603,7 +605,8 @@ Proof
   fs [] >>
   fs [state_rel_def, set_store_def,
       loopSemTheory.set_globals_def, globals_rel_def] >>
-  rw [FLOOKUP_UPDATE]
+  rw [FLOOKUP_UPDATE] >>
+  rw[] >> gvs[]
 QED
 
 Theorem acc_vars_acc'[local] =
@@ -1133,9 +1136,7 @@ Proof
     >- (
      fs [Abbr ‘ctxt’] >>
      match_mp_tac locals_rel_mk_ctxt_ln >>
-     fs []) >>
-    conj_tac >- fs[state_rel_def] >>
-    conj_tac >- fs[state_rel_def]
+     fs [])
     >> (
      fs [no_Loops_def, no_Loop_def] >>
      fs [every_prog_def]) >>
@@ -1174,9 +1175,7 @@ Proof
      >- (
       fs [Abbr ‘ctxt’] >>
       match_mp_tac locals_rel_mk_ctxt_ln >>
-      fs []) >>
-    conj_tac >- fs[state_rel_def] >>
-    conj_tac >- fs[state_rel_def]
+      fs [])
      >> (
       fs [no_Loops_def, no_Loop_def] >>
       fs [every_prog_def]) >>
@@ -1218,9 +1217,7 @@ Proof
    >- (
     fs [Abbr ‘ctxt’] >>
     match_mp_tac locals_rel_mk_ctxt_ln >>
-    fs []) >>
-    conj_tac >- fs[state_rel_def] >>
-    conj_tac >- fs[state_rel_def]
+    fs [])
      >> (
     fs [no_Loops_def, no_Loop_def] >>
     fs [every_prog_def]) >>
@@ -1260,9 +1257,7 @@ Proof
    >- (
     fs [Abbr ‘ctxt’] >>
     match_mp_tac locals_rel_mk_ctxt_ln >>
-    fs []) >>
-    conj_tac >- fs[state_rel_def] >>
-    conj_tac >- fs[state_rel_def]
+    fs [])
      >> (
     fs [no_Loops_def, no_Loop_def] >>
     fs [every_prog_def]) >>
@@ -1299,9 +1294,7 @@ Proof
    >- (
     fs [Abbr ‘ctxt’] >>
     match_mp_tac locals_rel_mk_ctxt_ln >>
-    fs []) >>
-    conj_tac >- fs[state_rel_def] >>
-    conj_tac >- fs[state_rel_def]
+    fs [])
      >> (
     fs [no_Loops_def, no_Loop_def] >>
     fs [every_prog_def]) >>
@@ -1375,8 +1368,6 @@ Proof
     fs [Abbr ‘ctxt’] >>
     match_mp_tac locals_rel_mk_ctxt_ln >>
     fs []) >>
-   impl_tac>- fs[state_rel_def] >>
-   impl_tac>- fs[state_rel_def] >>
    impl_tac >- (
     fs [no_Loops_def, no_Loop_def] >>
     fs [every_prog_def]) >>
@@ -1408,8 +1399,6 @@ Proof
    fs [Abbr ‘ctxt’] >>
    match_mp_tac locals_rel_mk_ctxt_ln >>
    fs []) >>
-   impl_tac>- fs[state_rel_def] >>
-   impl_tac>- fs[state_rel_def] >>
   impl_tac
   >- (
    fs [no_Loops_def, no_Loop_def] >>
@@ -1426,7 +1415,9 @@ Proof
                [‘Call NONE (SOME start) [0] NONE’, ‘t with clock := k’] mp_tac) >>
   strip_tac >> fs [] >>
   qexists_tac ‘k’ >> fs [] >>
-  fs [state_rel_def]
+  fs [state_rel_def] >>
+  first_x_assum drule >>
+  gvs[]
 QED
 
 Definition st_rel_def:
